Simulation relation for consistency

src/mapping/PStoRMWConsistent.v
@@ -46,6 +46,130 @@ Set Implicit Arguments.
 Module PStoRMWConsistent.
   Import PStoRMWThread.
 
+  Definition sim_val_cons (n: Time.t) (val_ps: Const.t) (val_arm: ValA.t (A:=View.t (A:=unit))): Prop :=
+    le val_arm.(ValA.annot).(View.ts) n -> sim_val val_ps val_arm.(ValA.val).
+
+  Definition sim_regs_cons (n: Time.t) (regs_ps: RegFile.t) (regs_arm: RMap.t (A:=View.t (A:=unit))): Prop :=
+    forall r, sim_val_cons n (IdentFun.find r regs_ps) (RMap.find r regs_arm).
+
+  Variant sim_state_cons (n: Time.t) (st_ps: State.t) (st_arm: RMWState.t (A:=View.t (A:=unit))): Prop :=
+    | sim_state_cons_intro
+        (STMTS: RMWState.stmts st_arm = ps_to_rmw_stmts (State.stmts st_ps))
+        (REGS: sim_regs_cons n st_ps.(State.regs) st_arm.(RMWState.rmap))
+  .
+  #[export] Hint Constructors sim_state: core.
+
+  Variant sim_memory_cons (tid: Ident.t) (n: Time.t)
+    (lc_ps: PSLocal.t) (gprm_ps: BoolMap.t) (mem_ps: PSMemory.t)
+    (lc_arm: Local.t (A:=unit)) (mem_arm: Memory.t): Prop :=
+    | sim_memory_intro
+        (PRM_SOUND: forall ts (PROMISED_ARM: Promises.lookup ts lc_arm.(Local.promises)),
+          exists msg_arm loc_ps from,
+            (<<GET_ARM: Memory.get_msg ts mem_arm = Some msg_arm>>) /\
+            (<<TID: msg_arm.(Msg.tid) = tid>>) /\
+            (<<LOC: msg_arm.(Msg.loc) = Zpos loc_ps>>) /\
+            (<<RESERVED: Memory.get loc_ps (ntt ts) (PSLocal.reserves lc_ps) = Some (from, Message.reserve)>>) /\
+            (<<PROMISED_PS: le ts n -> lc_ps.(PSLocal.promises) loc_ps = true>>))
+        (PRM_COMPLETE: forall loc (PROMISED_PS: lc_ps.(PSLocal.promises) loc = true),
+          exists ts msg_arm,
+            (<<LE: le ts n>>) /\
+            (<<PROMISED_ARM: Promises.lookup ts lc_arm.(Local.promises)>>) /\
+            (<<GET_ARM: Memory.get_msg ts mem_arm = Some msg_arm>>) /\
+            (<<LOC: msg_arm.(Msg.loc) = Zpos loc>>))
+        (MEM_SOUND: forall ts msg_arm
+                           (GET_ARM: Memory.get_msg ts mem_arm = Some msg_arm),
+          exists loc_ps from msg_ps,
+            (<<LOC: msg_arm.(Msg.loc) = Zpos loc_ps>>) /\
+            (<<GET_PS: PSMemory.get loc_ps (ntt ts) mem_ps = Some (from, msg_ps)>>) /\
+            (<<TS: PSTime.lt from (ntt ts)>>) /\
+            (__guard__ (
+               (<<FROM: from = PSTime.bot>>) \/
+               exists fts fval ftid,
+                 (<<FROM: from = ntt fts>>) /\
+                 (<<GET_FROM_ARM: Memory.get_msg fts mem_arm = Some (Msg.mk msg_arm.(Msg.loc) fval ftid)>>) /\
+                 (<<LATEST: Memory.latest msg_arm.(Msg.loc) fts ts mem_arm>>))) /\
+            (__guard__ (
+               (<<MSG: msg_ps = Message.reserve>>) /\
+               (<<PROMISED_ARM: Promises.lookup ts lc_arm.(Local.promises) <-> msg_arm.(Msg.tid) = tid>>) /\
+               (<<PROMISED: le ts n ->
+                            (<<GPROMISED: gprm_ps loc_ps = true>>) /\
+                            (<<PROMISED_PS: lc_ps.(PSLocal.promises) loc_ps <-> msg_arm.(Msg.tid) = tid>>)>>) \/
+               exists val_ps released na,
+                 (<<MSG: msg_ps = Message.message val_ps released na>>) /\
+                 (<<VAL: le ts n -> sim_val val_ps msg_arm.(Msg.val)>>) /\
+                 (<<PROMISED_ARM: Promises.lookup ts lc_arm.(Local.promises) = false>>))))
+        (MEM_COMPLETE: forall loc_ps from to msg_ps
+                              (TO: PSTime.lt PSTime.bot to)
+                              (GET_PS: PSMemory.get loc_ps to mem_ps = Some (from, msg_ps)),
+          (exists fts,
+              (<<FROM: from = ntt fts>>) /\
+              (<<OUT: forall ts msg_arm
+                        (LE: le fts ts)
+                        (GET_ARM: Memory.get_msg ts mem_arm = Some msg_arm),
+                  msg_arm.(Msg.loc) <> Zpos loc_ps>>)) \/
+          exists ts msg_arm,
+            (<<TO: to = ntt ts>>) /\
+            (<<GET_ARM: Memory.get_msg ts mem_arm = Some msg_arm>>) /\
+            (<<LOC: msg_arm.(Msg.loc) = Zpos loc_ps>>))
+        (FWD: forall loc ts (FWD: (lc_arm.(Local.fwdbank) loc).(FwdItem.ts) = ts),
+            exists loc_ps from val released na,
+              (<<LOC: loc = Zpos loc_ps>>) /\
+              (<<GET_PS: PSMemory.get loc_ps (ntt ts) mem_ps = Some (from, Message.message val released na)>>) /\
+              (<<REL_FWD: if (lc_arm.(Local.fwdbank) loc).(FwdItem.ex)
+                          then forall loc, PSTime.le
+                                        ((PSView.unwrap released).(View.rlx) loc)
+                                        (ntt (View.ts (join (join lc_arm.(Local.vrn) lc_arm.(Local.vro))
+                                                            (lc_arm.(Local.coh) (Zpos loc)))))
+                            (* PSView.opt_le released (Some lc_ps.(PSLocal.tview).(PSTView.acq)) *)
+                          else PSView.le (View.unwrap released) (lc_ps.(PSLocal.tview).(PSTView.rel) loc_ps)>>))
+        (RELEASED: forall loc from to val released na
+                          (GET: PSMemory.get loc to mem_ps = Some (from, Message.message val released na)),
+          forall loc', PSTime.le ((View.unwrap released).(View.rlx) loc') to)
+  .
+
+  Variant sim_thread_cons (tid: Ident.t) (n: Time.t)
+    (th_ps: PSThread.t lang_ps) (eu: RMWExecUnit.t (A:=unit)): Prop :=
+    | sim_thread_cons_intro
+        (SIM_STATE: sim_state_cons n (PSThread.state th_ps) (RMWExecUnit.state eu))
+        (SIM_TVIEW: sim_tview (PSLocal.tview (PSThread.local th_ps)) (RMWExecUnit.local eu))
+        (SIM_MEM: sim_memory_cons tid n
+                                  (PSThread.local th_ps)
+                                  (PSGlobal.promises (PSThread.global th_ps))
+                                  (PSGlobal.memory (PSThread.global th_ps))
+                                  (RMWExecUnit.local eu) (RMWExecUnit.mem eu))
+  .
+
+  Lemma sim_regs_cons_eval_expr
+        n regs_ps regs_arm e
+        (SIM: sim_regs_cons n regs_ps regs_arm):
+    sim_val_cons n (RegFile.eval_expr regs_ps e) (sem_expr regs_arm (ps_to_rmw_expr e)).
+  Proof.
+    induction e; ss.
+    - ii. exploit IHe; eauto. i.
+      destruct op. ss. inv x0; ss.
+      condtac; econs.
+    - ii. ss.
+      exploit IHe1; [etrans; eauto; apply join_l|]. i.
+      exploit IHe2; [etrans; eauto; apply join_r|]. i.
+      destruct op; inv x0; inv x1; ss.
+  Qed.
+
+  Lemma sim_regs_cons_add
+        n regs_ps regs_arm
+        r val_ps (val_arm: ValA.t (A:=View.t (A:=unit)))
+        (SIM: sim_regs_cons n regs_ps regs_arm)
+        (VAL: sim_val_cons n val_ps val_arm):
+    sim_regs_cons n (IdentFun.add r val_ps regs_ps)
+                  (RMap.add r val_arm regs_arm).
+  Proof.
+    ii. rewrite IdentFun.add_spec, RMap.add_o.
+    condtac; ss; subst.
+    - condtac; try congr.
+      revert H. rewrite RMap.add_o. condtac; ss.
+    - condtac; ss. apply SIM.
+      revert H. rewrite RMap.add_o. condtac; ss.
+  Qed.
+
   Lemma sim_thread_exec_consistent
         tid n after_sc th1_ps eu
         (SIM1: sim_thread_exec tid n after_sc th1_ps eu)
